ProofLibrary/TermBasics.lean
@@ -56,31 +56,29 @@ inductive VarOrConst (sig : Signature) [DecidableEq sig.C] [DecidableEq sig.V] w
 
 variable {sig : Signature} [DecidableEq sig.C] [DecidableEq sig.V]
 
-def PreGroundTerm.contains_func (func : SkolemFS sig) : PreGroundTerm sig -> Bool
-| .leaf _ => false
-| .inner func' ts => func == func' || ts.toList.attach.any (fun ⟨t, mem⟩ =>
-  have : t.depth < (FiniteTree.inner func' ts).depth := by
-    conv => right; unfold FiniteTree.depth
-    rw [Nat.add_comm]
-    apply Nat.lt_add_one_of_le
-    apply FiniteTree.depth_le_depthList_of_mem
-    exact mem
-  contains_func func t
-)
-termination_by t => FiniteTree.depth t
+mutual
 
-def PreGroundTerm.cyclic : PreGroundTerm sig -> Bool
-| .leaf _ => false
-| .inner func ts => (ts.toList.any (contains_func func)) || ts.toList.attach.any (fun ⟨t, mem⟩ =>
-  have : t.depth < (FiniteTree.inner func ts).depth := by
-    conv => right; unfold FiniteTree.depth
-    rw [Nat.add_comm]
-    apply Nat.lt_add_one_of_le
-    apply FiniteTree.depth_le_depthList_of_mem
-    exact mem
-  cyclic t
-)
-termination_by t => FiniteTree.depth t
+  def PreGroundTerm.contains_func (func : SkolemFS sig) : FiniteTree (SkolemFS sig) sig.C -> Bool
+  | .leaf _ => false
+  | .inner func' ts => func == func' || PreGroundTerm.contains_func_list func ts
+
+  def PreGroundTerm.contains_func_list (func : SkolemFS sig) : FiniteTreeList (SkolemFS sig) sig.C -> Bool
+  | .nil => false
+  | .cons hd tl => contains_func func hd || contains_func_list func tl
+
+end
+
+mutual
+
+  def PreGroundTerm.cyclic : FiniteTree (SkolemFS sig) sig.C -> Bool
+  | .leaf _ => false
+  | .inner func ts => (contains_func_list func ts) || PreGroundTerm.cyclic_list ts
+
+  def PreGroundTerm.cyclic_list : FiniteTreeList (SkolemFS sig) sig.C -> Bool
+  | .nil => false
+  | .cons hd tl => PreGroundTerm.cyclic hd || PreGroundTerm.cyclic_list tl
+
+end
 
 def GroundTerm.const (c : sig.C) : GroundTerm sig := ⟨FiniteTree.leaf c, by simp [PreGroundTerm.arity_ok]⟩
 def GroundTerm.func (func : SkolemFS sig) (ts : List (GroundTerm sig)) (arity_ok : ts.length = func.arity) : GroundTerm sig := ⟨FiniteTree.inner func (FiniteTreeList.fromList ts.unattach), by
@@ -681,3 +679,289 @@ section ListsOfTerms
                 rw [eq]
 
 end ListsOfTerms
+
+mutual
+
+  def PreGroundTerm.function_paths : FiniteTree (SkolemFS sig) sig.C -> List (List (SkolemFS sig))
+  | .leaf _ => [[]]
+  | .inner f ts =>
+    match ts with
+    | .nil => [[f]]
+    | _ => (function_paths_list ts).map (fun path => f :: path)
+
+  def PreGroundTerm.function_paths_list : FiniteTreeList (SkolemFS sig) sig.C -> List (List (SkolemFS sig))
+  | .nil => []
+  | .cons hd tl => (function_paths hd) ++ (function_paths_list tl)
+
+end
+
+mutual
+
+  theorem PreGroundTerm.function_path_elements_are_inner_labels (t : FiniteTree (SkolemFS sig) sig.C) : ∀ (path : List (SkolemFS sig)), path ∈ PreGroundTerm.function_paths t -> ∀f, f ∈ path -> f ∈ t.innerLabels := by
+    intro path path_mem f f_mem
+    cases t with
+    | leaf c =>
+      simp only [function_paths, List.mem_singleton] at path_mem
+      rw [path_mem] at f_mem
+      simp at f_mem
+    | inner func ts =>
+      unfold function_paths at path_mem
+      cases ts with
+      | nil =>
+        rw [List.mem_singleton] at path_mem
+        rw [path_mem] at f_mem
+        rw [List.mem_singleton] at f_mem
+        unfold FiniteTree.innerLabels
+        rw [List.mem_cons]
+        apply Or.inl
+        exact f_mem
+      | cons hd tl =>
+        rw [List.mem_map] at path_mem
+        rcases path_mem with ⟨path', mem, eq⟩
+        rw [← eq] at f_mem
+        rw [List.mem_cons] at f_mem
+        unfold FiniteTree.innerLabels
+        rw [List.mem_cons]
+        cases f_mem with
+        | inl f_mem => apply Or.inl; exact f_mem
+        | inr f_mem =>
+          apply Or.inr
+          exact function_path_elements_are_inner_labels_list (FiniteTreeList.cons hd tl) path' mem f f_mem
+
+  theorem PreGroundTerm.function_path_elements_are_inner_labels_list (ts : FiniteTreeList (SkolemFS sig) sig.C) : ∀ (path : List (SkolemFS sig)), path ∈ PreGroundTerm.function_paths_list ts -> ∀f, f ∈ path -> f ∈ FiniteTree.innerLabelsList ts := by
+    intro path path_mem f f_mem
+    cases ts with
+    | nil =>
+      unfold function_paths_list at path_mem
+      simp at path_mem
+    | cons hd tl =>
+      unfold function_paths_list at path_mem
+      rw [List.mem_append] at path_mem
+      unfold FiniteTree.innerLabelsList
+      rw [List.mem_append]
+      cases path_mem with
+      | inl path_mem =>
+        apply Or.inl
+        exact function_path_elements_are_inner_labels hd path path_mem f f_mem
+      | inr path_mem =>
+        apply Or.inr
+        exact function_path_elements_are_inner_labels_list tl path path_mem f f_mem
+
+end
+
+mutual
+
+  theorem PreGroundTerm.function_path_of_depth_exists (t : FiniteTree (SkolemFS sig) sig.C) : ∃ (path : List (SkolemFS sig)), path ∈ PreGroundTerm.function_paths t ∧ path.length = t.depth - 1 := by
+    cases t with
+    | leaf c => exists []; simp [FiniteTree.depth, function_paths]
+    | inner f ts =>
+      cases ts with
+      | nil =>
+        exists [f]
+        constructor
+        . unfold function_paths
+          simp
+        . unfold FiniteTree.depth
+          unfold FiniteTree.depthList
+          simp
+      | cons hd tl =>
+        rcases PreGroundTerm.function_path_of_depth_exists_list (FiniteTreeList.cons hd tl) (by simp) with ⟨path, mem, len⟩
+        exists (f :: path)
+        constructor
+        . unfold function_paths
+          rw [List.mem_map]
+          exists path
+        . unfold List.length
+          unfold FiniteTree.depth
+          rw [len]
+          rw [Nat.sub_one_add_one]
+          . rw [Nat.add_comm]
+            simp
+          . unfold FiniteTree.depthList
+            intro contra
+            have : hd.depth = 0 ∧ FiniteTree.depthList tl = 0 := by omega
+            have contra := this.left
+            unfold FiniteTree.depth at contra
+            cases hd <;> simp at contra
+
+  theorem PreGroundTerm.function_path_of_depth_exists_list (ts : FiniteTreeList (SkolemFS sig) sig.C) : ts ≠ FiniteTreeList.nil -> ∃ (path : List (SkolemFS sig)), path ∈ PreGroundTerm.function_paths_list ts ∧ path.length = (FiniteTree.depthList ts) - 1 := by
+    intro neq
+    cases ts with
+    | nil => simp at neq
+    | cons hd tl =>
+      cases tl with
+      | nil =>
+        have := function_path_of_depth_exists hd
+        rcases this with ⟨path, mem, len⟩
+        exists path
+        constructor
+        . unfold function_paths_list
+          rw [List.mem_append]
+          apply Or.inl
+          exact mem
+        . unfold FiniteTree.depthList
+          unfold FiniteTree.depthList
+          rw [Nat.max_eq_left]
+          . exact len
+          . unfold FiniteTree.depth
+            cases hd <;> simp
+      | cons mid tl =>
+        cases Decidable.em (hd.depth ≤ FiniteTree.depthList (FiniteTreeList.cons mid tl)) with
+        | inl depth_le =>
+          have := PreGroundTerm.function_path_of_depth_exists_list (FiniteTreeList.cons mid tl) (by simp)
+          rcases this with ⟨path, mem, len⟩
+          exists path
+          constructor
+          . unfold function_paths_list
+            rw [List.mem_append]
+            apply Or.inr
+            exact mem
+          . unfold FiniteTree.depthList
+            rw [Nat.max_eq_right]
+            . exact len
+            . exact depth_le
+        | inr depth_le =>
+          have := function_path_of_depth_exists hd
+          rcases this with ⟨path, mem, len⟩
+          exists path
+          constructor
+          . unfold function_paths_list
+            rw [List.mem_append]
+            apply Or.inl
+            exact mem
+          . unfold FiniteTree.depthList
+            rw [Nat.max_eq_left]
+            . exact len
+            . apply Nat.le_of_lt
+              simp at depth_le
+              exact depth_le
+
+end
+
+mutual
+
+  theorem PreGroundTerm.function_path_elements_are_in_contains_func (t : FiniteTree (SkolemFS sig) sig.C) : ∀ (path : List (SkolemFS sig)), path ∈ PreGroundTerm.function_paths t -> ∀f, f ∈ path -> PreGroundTerm.contains_func f t := by
+    intro path path_mem f f_mem
+    cases t with
+    | leaf c =>
+      simp only [function_paths, List.mem_singleton] at path_mem
+      rw [path_mem] at f_mem
+      simp at f_mem
+    | inner func ts =>
+      unfold contains_func
+      rw [Bool.or_eq_true]
+      unfold function_paths at path_mem
+      cases ts with
+      | nil =>
+        rw [List.mem_singleton] at path_mem
+        rw [path_mem] at f_mem
+        rw [List.mem_singleton] at f_mem
+        apply Or.inl
+        rw [f_mem]
+        simp
+      | cons hd tl =>
+        rw [List.mem_map] at path_mem
+        rcases path_mem with ⟨path', mem, eq⟩
+        rw [← eq] at f_mem
+        rw [List.mem_cons] at f_mem
+        cases f_mem with
+        | inl f_mem => apply Or.inl; rw [f_mem]; simp
+        | inr f_mem =>
+          apply Or.inr
+          exact PreGroundTerm.function_path_elements_are_in_contains_func_list (FiniteTreeList.cons hd tl) path' mem f f_mem
+
+  theorem PreGroundTerm.function_path_elements_are_in_contains_func_list (ts : FiniteTreeList (SkolemFS sig) sig.C) : ∀ (path : List (SkolemFS sig)), path ∈ PreGroundTerm.function_paths_list ts -> ∀f, f ∈ path -> PreGroundTerm.contains_func_list f ts := by
+    intro path path_mem f f_mem
+    cases ts with
+    | nil =>
+      unfold function_paths_list at path_mem
+      simp at path_mem
+    | cons hd tl =>
+      unfold contains_func_list
+      rw [Bool.or_eq_true]
+      unfold function_paths_list at path_mem
+      rw [List.mem_append] at path_mem
+      cases path_mem with
+      | inl path_mem => apply Or.inl; exact function_path_elements_are_in_contains_func hd path path_mem f f_mem
+      | inr path_mem => apply Or.inr; exact function_path_elements_are_in_contains_func_list tl path path_mem f f_mem
+
+end
+
+mutual
+
+  theorem PreGroundTerm.cyclic_of_path_with_dup (t : FiniteTree (SkolemFS sig) sig.C) (path : List (SkolemFS sig)) (path_mem : path ∈ PreGroundTerm.function_paths t) (dup : ¬ path.Nodup) : PreGroundTerm.cyclic t := by
+    cases t with
+    | leaf c =>
+      unfold PreGroundTerm.function_paths at path_mem
+      rw [List.mem_singleton] at path_mem
+      rw [path_mem] at dup
+      simp at dup
+    | inner f ts =>
+      unfold PreGroundTerm.function_paths at path_mem
+      cases ts with
+      | nil =>
+        rw [List.mem_singleton] at path_mem
+        rw [path_mem] at dup
+        simp at dup
+      | cons hd tl =>
+        rw [List.mem_map] at path_mem
+        rcases path_mem with ⟨path', mem, eq⟩
+        unfold PreGroundTerm.cyclic
+        rw [Bool.or_eq_true]
+        cases Decidable.em (f ∈ path') with
+        | inl f_mem =>
+          apply Or.inl
+          exact PreGroundTerm.function_path_elements_are_in_contains_func_list (FiniteTreeList.cons hd tl) path' mem f f_mem
+        | inr f_mem =>
+          apply Or.inr
+          rw [← eq] at dup
+          rw [List.nodup_cons] at dup
+          simp only [not_and] at dup
+          apply PreGroundTerm.cyclic_of_path_with_dup_list (FiniteTreeList.cons hd tl) path' mem
+          apply dup
+          apply f_mem
+
+  theorem PreGroundTerm.cyclic_of_path_with_dup_list (ts : FiniteTreeList (SkolemFS sig) sig.C) (path : List (SkolemFS sig)) (path_mem : path ∈ PreGroundTerm.function_paths_list ts) (dup : ¬ path.Nodup) : PreGroundTerm.cyclic_list ts := by
+    unfold cyclic_list
+    cases ts with
+    | nil =>
+      unfold PreGroundTerm.function_paths_list at path_mem
+      simp at path_mem
+    | cons hd tl =>
+      unfold PreGroundTerm.function_paths_list at path_mem
+      rw [List.mem_append] at path_mem
+      rw [Bool.or_eq_true]
+      cases path_mem with
+      | inl path_mem =>
+        apply Or.inl
+        exact cyclic_of_path_with_dup hd path path_mem dup
+      | inr path_mem =>
+        apply Or.inr
+        exact cyclic_of_path_with_dup_list tl path path_mem dup
+
+end
+
+theorem PreGroundTerm.cyclic_of_depth_too_big (t : PreGroundTerm sig) (funcs : List (SkolemFS sig)) (nodup : funcs.Nodup) (funcs_in_t_from_funcs : ∀ func, func ∈ t.innerLabels -> func ∈ funcs) : funcs.length + 2 ≤ t.depth -> PreGroundTerm.cyclic t := by
+  intro le_depth
+  have := PreGroundTerm.function_path_of_depth_exists t
+  rcases this with ⟨path, path_mem, path_len⟩
+
+  have path_length_gt : funcs.length < path.length := by
+    rw [path_len]
+    apply Nat.lt_of_succ_le
+    apply Nat.le_of_succ_le_succ
+    rw [Nat.succ_eq_add_one]
+    rw [Nat.succ_eq_add_one]
+    rw [Nat.sub_one_add_one]
+    . exact le_depth
+    . unfold FiniteTree.depth
+      cases t <;> simp
+
+  have dup_in_path : ¬ path.Nodup := by
+    apply List.contains_dup_of_exceeding_nodup_list_with_same_elements funcs path nodup path_length_gt
+    intro f f_mem
+    apply funcs_in_t_from_funcs
+    exact PreGroundTerm.function_path_elements_are_inner_labels t path path_mem f f_mem
+
+  exact PreGroundTerm.cyclic_of_path_with_dup t path path_mem dup_in_path
+
